wip

SSA/Experimental/Context.lean
@@ -4,17 +4,20 @@ import Mathlib.Tactic
 inductive Ty
   | nat
   | bool
+  | fn : Ty → Ty → Ty
   deriving DecidableEq, Repr
 
 @[reducible]
 def Ty.toType
   | nat => Nat
   | bool => Bool
+  | fn a b => a.toType → b.toType
 
 
 
 def Ctxt : Type :=
   List Ty
+  deriving DecidableEq
 
 namespace Ctxt
 
@@ -44,8 +47,8 @@ def emptyElim {α : Sort _} {t : Ty} : Ctxt.Var ∅ t → α :=
 /-- Take a variable in a context `Γ` and get the corresponding variable
 in context `Γ.snoc t`. This is marked as a coercion. -/
 @[coe]
-def toSnoc {Γ : Ctxt} {t t' : Ty} (var : Ctxt.Var Γ t) : Ctxt.Var (Ctxt.snoc Γ t') t  :=
-  ⟨var.1+1, by cases var; simp_all⟩
+def toSnoc {Γ : Ctxt} {t' : Ty} ⦃t⦄ (var : Ctxt.Var Γ t) : Ctxt.Var (Ctxt.snoc Γ t') t  :=
+  ⟨var.1+1, by cases var; simp_all[snoc]⟩
   
 /-- This is an induction principle that case splits on whether or not a variable 
 is the last variable in a context. -/
@@ -92,31 +95,39 @@ end Var
 
 section Append
 
-def append : Ctxt → Ctxt → Ctxt :=
-  fun xs ys => List.append ys xs
+instance instAppend : Append (Ctxt) where
+  append Γ₁ Γ₂ := List.append Γ₂ Γ₁
 
+instance : HasSubset (Ctxt) where
+  Subset Γ₁ Γ₂ := ∃ Δ, Γ₂ = Γ₁ ++ Δ
 
-theorem append_empty (Γ : Ctxt) : append Γ ∅ = Γ := by
-  simp[append, EmptyCollection.emptyCollection, empty]
+def drop : Nat → Ctxt → Ctxt := List.drop
+
+theorem append_empty (Γ : Ctxt) : Γ ++ ∅ = Γ := by
+  show List.append [] Γ = Γ  
+  simp
   
 
 theorem append_snoc (Γ Γ' : Ctxt) (t : Ty) : 
-    append Γ (Ctxt.snoc Γ' t) = (append Γ Γ').snoc t := by
-  simp[append, snoc]
+    Γ ++ (Ctxt.snoc Γ' t) = (Γ ++ Γ').snoc t := by
+  show List.append (Ctxt.snoc Γ' t) Γ = snoc (List.append Γ' Γ) t
+  simp only [snoc, List.append]
 
 @[simp]
 theorem _root_.List.get?_append_add :
     List.get? (xs ++ ys) (i + xs.length) = List.get? ys i := by
   induction xs
   . rfl
-  . simp_all
+  next ih =>
+    simp[List.get?]
+    apply ih
 
-def Var.inl {Γ Γ' : Ctxt} {t : Ty} : Var Γ t → Var (Ctxt.append Γ Γ') t
-  | ⟨v, h⟩ => ⟨v + Γ'.length, by simp[←h, append, List.get?_append_add]⟩
+def Var.inl {Γ Γ' : Ctxt} {t : Ty} : Var Γ t → Var (Γ ++ Γ') t
+  | ⟨v, h⟩ => ⟨v + Γ'.length, by simp[←h, (· ++ ·), Append.append, List.get?_append_add]⟩
 
-def Var.inr {Γ Γ' : Ctxt} {t : Ty} : Var Γ' t → Var (append Γ Γ') t
+def Var.inr {Γ Γ' : Ctxt} {t : Ty} : Var Γ' t → Var (Γ ++ Γ') t
   | ⟨v, h⟩ => ⟨v, by 
-      simp[append]
+      simp[(· ++ ·), Append.append]
       induction Γ' generalizing v
       case nil =>
         contradiction
@@ -127,6 +138,40 @@ def Var.inr {Γ Γ' : Ctxt} {t : Ty} : Var Γ' t → Var (append Γ Γ') t
         case succ v =>
           apply ih v h
     ⟩
+
+def Var.appendSplit {Γ₁} : Var (Γ₁ ++ Γ₂) t → (Var Γ₁ t) ⊕ (Var Γ₂ t) :=
+  fun v => match Γ₂, v with 
+    | [], v => .inl v
+    | _::_, ⟨0, h⟩ => .inr ⟨0, h⟩
+    | _::Γ, ⟨v+1, h⟩ => 
+      match appendSplit (Γ₂:=Γ) ⟨v, h⟩ with
+        | .inl v => .inl v
+        | .inr v => .inr v.toSnoc
+
+
+def Ctxt.subset_diff {Γ₁ Γ₂ : Ctxt} (h : Γ₁ ⊆ Γ₂) : {Δ : Ctxt // Γ₂ = Γ₁ ++ Δ} :=
+  sorry
+
+def Var.weaken {Γ₁ Γ₂ : Ctxt} {t} (h : Γ₁ ⊆ Γ₂) (v : Γ₁.Var t) : Γ₂.Var t :=
+  let ⟨Δ, hΔ⟩ := Ctxt.subset_diff h
+  hΔ ▸ @Var.inl Γ₁ Δ _ v
+  
+
+def hom (Γ₁ Γ₂ : Ctxt) : Type :=
+  ⦃t : Ty⦄ → Γ₁.Var t → Γ₂.Var t
+
+
+@[coe]
+def hom.toSnocRight {Γ₁ Γ₂ : Ctxt} (f : Γ₁.hom Γ₂) : Γ₁.hom (Γ₂.snoc t) :=
+  fun _ v => (f v).toSnoc
+
+def hom.toSnoc {Γ₁ Γ₂ : Ctxt} (f : Γ₁.hom Γ₂) : (Γ₁.snoc t).hom (Γ₂.snoc t) :=
+  fun _ v => by 
+    cases v using Ctxt.Var.casesOn with
+    | last => exact .last ..
+    | base v => exact .toSnoc <| f v
+
+
 
 end Append
 
