SSA/Experimental/Hoas.lean
@@ -1,0 +1,52 @@
+import SSA.Core.WellTypedFramework
+import SSA.Experimental.Context
+
+namespace SSA
+
+inductive Ty 
+  | nat
+  deriving DecidableEq, Repr
+
+def Ty.toType : Ty → Type
+  | .nat => Nat
+
+
+/-- A very simple intrinsically typed expression. -/
+inductive IExpr : Ctxt → Ty → Type
+  | add (a b : Γ.Var .nat) : IExpr Γ .nat
+  /-- Nat literals. -/
+  | nat (n : Nat) : IExpr Γ .nat
+
+/-- A very simple intrinsically typed program: a sequence of let bindings. -/
+inductive ICom : Ctxt →  Ty → Type where
+  | ret {Γ : Ctxt} : Γ.Var t → ICom Γ t
+  | lete (e : IExpr Γ α) (body : ICom (Γ.snoc α) β) : ICom Γ β
+
+
+
+
+class HOAS (expr stmt var : Ty → Type) where
+  /-- let-binding -/
+  assign {T : Ty} (rhs : expr T) 
+      (rest : var T → stmt T')
+      : stmt T'
+  -- /-- above; ret v -/
+  ret (v : expr T) : stmt T
+  add (a b : var (.nat)) : expr (.nat)
+
+def HOASExpr : Type := ∀ (expr stmt var : Ty → Type) [HOAS expr stmt var], expr
+def HOASCom : Type := ∀ (expr stmt var : Ty → Type) [HOAS expr stmt var], stmt
+def HOASVar : Type := ∀ (expr stmt var : Ty → Type) [HOAS expr stmt var], var
+
+
+
+
+def IExpr.fromHOAS : HOASExpr t → IExpr ∅ t := 
+  sorry
+
+
+def TSSA.fromHOAS : 
+
+
+
+end SSA
